vale/specs/hardware/X64.Leakage_s.fst
@@ -53,14 +53,22 @@ let isConstantTime (code:tainted_code) (ts:taintState) =
   forall s1 s2 fuel.
       isConstantTimeGivenStates code fuel ts s1 s2
 
-let isExplicitLeakageFreeGivenStates (code:tainted_code) (fuel:nat) (ts:taintState) (ts':taintState) (s1:traceState) (s2:traceState) =
-  let r1 = taint_eval_code code fuel s1 in
-  let r2 = taint_eval_code code fuel s2 in
- ( Some? r1 /\ Some? r2
-  /\ s1.state.ok /\ (Some?.v r1).state.ok
-  /\ s2.state.ok /\ (Some?.v r2).state.ok
-  /\ constTimeInvariant ts s1 s2
- ) ==> publicValuesAreSame ts' (Some?.v r1) (Some?.v r2)
+let is_explicit_leakage_free_lhs (code:tainted_code) (fuel:nat)
+                                 (ts:taintState) (ts':taintState) (s1:traceState) (s2:traceState)
+  = s1.state.ok /\ s2.state.ok /\ constTimeInvariant ts s1 s2 /\
+    (let r1 = taint_eval_code code fuel s1 in
+     let r2 = taint_eval_code code fuel s2 in
+     Some? r1 /\ Some? r2 /\ (Some?.v r1).state.ok /\ (Some?.v r2).state.ok)
+
+let is_explicit_leakage_free_rhs (code:tainted_code) (fuel:nat)
+                                 (ts:taintState) (ts':taintState) (s1:traceState) (s2:traceState)
+  = let r1 = taint_eval_code code fuel s1 in
+    let r2 = taint_eval_code code fuel s2 in
+    Some? r1 /\ Some? r2 /\ publicValuesAreSame ts' (Some?.v r1) (Some?.v r2)
+
+let isExplicitLeakageFreeGivenStates (code:tainted_code) (fuel:nat)
+                                     (ts:taintState) (ts':taintState) (s1:traceState) (s2:traceState)
+  = is_explicit_leakage_free_lhs code fuel ts ts' s1 s2 ==> is_explicit_leakage_free_rhs code fuel ts ts' s1 s2
 
 let isExplicitLeakageFree (code:tainted_code) (ts:taintState) (ts':taintState) =
   forall s1 s2 fuel.
