vale/specs/hardware/X64.Machine_s.fst
@@ -65,4 +65,4 @@ type observation:eqtype =
   | MemAccess: addr:nat64 -> observation
   | MemAccessOffset: base:nat64 -> index:nat64 -> observation
 
-type memTaint_t = (m:Map.t int taint{Map.domain m == Set.complement Set.empty})
+type memTaint_t = (m:Map.t int taint{Set.equal (Map.domain m) (Set.complement Set.empty)})
